{
 "cells": [
  {
   "attachments": {},
   "cell_type": "markdown",
   "metadata": {},
   "source": [
    "# Exponential methods"
   ]
  },
  {
   "attachments": {},
   "cell_type": "markdown",
   "metadata": {},
   "source": [
    "Here is used informations from [1], [6], [7]."
   ]
  },
  {
   "attachments": {},
   "cell_type": "markdown",
   "metadata": {},
   "source": [
    "## Exponential Euler method\n",
    "\n",
    "For\n",
    "\n",
    "$\\begin{cases}\n",
    "    y'(t) + \\lambda y(t) = g(y(t), t), t \\in (t_0, T) \\\\\n",
    "    y(0) = y_0\n",
    "\\end{cases}$\n",
    "\n",
    "the domain is evenly discretized:\n",
    "\n",
    "$$\n",
    "    N \\in \\mathbb{N}; h = \\frac{T-t_0}{N}; \\text{Domain: }\\{t_k = t_0 + k h : k = 0, 1, ...\\}.\n",
    "$$\n",
    "\n",
    "The discretization of the ODE takes the exact solution of the Cauchy problem, given by the variation of constants formula\n",
    "\n",
    "$$\n",
    "    y(t) = e^{-(t-t_0) \\lambda}y_0 + \\int_{t_0}^t [e^{-\\lambda(t-\\tau)} g(y(\\tau), \\tau)] d\\tau\n",
    "$$\n",
    "\n",
    "and, by Taylor expansion on $g$:\n",
    "\n",
    "$\\tau \\in (t_k, t_{k+1})$\n",
    "\n",
    "$$\n",
    "    g(y(\\tau), \\tau) = g(y(t_k), t_k) + (\\tau - t_k) \\frac{dg}{dt} (y(\\theta_k), \\theta_k)\n",
    "$$\n",
    "\n",
    "for a $\\theta_k \\in (t_k, t_{k+1}),$\n",
    "\n",
    "$$\n",
    "    y(t_{k+1}) = e^{-(t_{k+1}-t_k) \\lambda}y(t_k) + \\int_{t_k}^{t_{k+1}} [e^{-\\lambda(t_{k+1}-\\tau)} g(y(\\tau), \\tau)] d\\tau\n",
    "$$\n",
    "\n",
    "$$\n",
    "    = e^{-h \\lambda}y(t_k) + \\int_{t_k}^{t_{k+1}} \\left[e^{-\\lambda(t_{k+1}-\\tau)} \\left( g(y(t_k), t_k) + (\\tau - t_k) \\frac{dg}{dt} (y(\\theta_k), \\theta_k)\\right)\\right] d\\tau\n",
    "$$\n",
    "\n",
    "$$\n",
    "    = e^{-h \\lambda}y(t_k) + g(y(t_k), t_k) \\int_{t_k}^{t_{k+1}} e^{-\\lambda(t_{k+1}-\\tau)} d\\tau + \\frac{dg}{dt} (y(\\theta_k), \\theta_k) \\int_{t_k}^{t_{k+1}} (\\tau - t_k) e^{-\\lambda(t_{k+1}-\\tau)} d\\tau.\n",
    "$$\n",
    "\n",
    "Since\n",
    "\n",
    "$$\n",
    "    \\int_{t_k}^{t_{k+1}} e^{-\\lambda(t_{k+1}-\\tau)} d\\tau = h\\phi_1(-\\lambda h)= \\frac{1-e^{-h \\lambda}}{\\lambda}\n",
    "$$\n",
    "\n",
    "and, by the Taylor expansion of $e^{-\\lambda h}$ in the point zero\n",
    "\n",
    "$$\n",
    "    e^{-\\lambda h} = 1 - \\lambda h + \\frac{1}{2}\\lambda^2h^2 - \\frac{1}{3!}\\lambda^3h^3 + \\dotsi + \\frac{1}{n!} (-\\lambda h)^n + \\dotsi, n \\in \\mathbb{N}\n",
    "$$\n",
    "\n",
    "$$\n",
    "     \\int_{t_k}^{t_{k+1}} (\\tau - t_k) e^{-\\lambda(t_{k+1}-\\tau)} d\\tau =\n",
    "     h^2 \\phi_2 (-\\lambda h) =\n",
    "     h \\frac{\\phi_1(0) - \\phi_1(-\\lambda h)}{\\lambda} =\n",
    "     \\frac{h}{\\lambda} - \\frac{1-e^{-h \\lambda}}{\\lambda^2} = \\\\\n",
    "     \\frac{h}{\\lambda} - \\frac{1-(1 - \\lambda h + \\frac{1}{2}\\lambda^2h^2 - \\frac{1}{3!}\\lambda^3h^3 + \\dotsi + \\frac{1}{n!} (-\\lambda h)^n + \\dotsi)}{\\lambda^2} = \\\\\n",
    "     \\frac{h^2}{2} - \\frac{h^3}{3!} \\lambda + \\dotsi + \\frac{h^n}{n!} (-\\lambda)^{n-2} + \\dotsi  =  O(h^2),\n",
    "$$\n",
    "\n",
    "$$\n",
    "    y(t_{k+1}) = e^{-h \\lambda}y(t_k) + g(y(t_k), t_k) \\frac{1-e^{-h \\lambda}}{\\lambda} + \\frac{dg}{dt} (y(\\theta_k), \\theta_k) O(h^2),\n",
    "$$\n",
    "\n",
    "$$\n",
    "  y(t_{k+1}) = e^{-h \\lambda}y(t_k) + g(y(t_k), t_k) \\frac{1-e^{-h \\lambda}}{\\lambda} + O(h^2).\n",
    "$$\n",
    "\n",
    "That inspires the $\\textbf{Exponential Euler method}$ :\n",
    "\n",
    "$$\n",
    "y_0 = y(t_0)\\\\\n",
    "\\textbf{for } k = 0, 1, 2, ..., N-1 :\\\\\n",
    "    y_{k+1} = e^{-h \\lambda}y_k + g(y_k, t_k) \\frac{1-e^{-h \\lambda}}{\\lambda}\\\\\n",
    "    t_{k+1} = t_k + h\n",
    "$$\n",
    "\n",
    "with $y_k \\thickapprox y(t_k)$."
   ]
  },
  {
   "attachments": {},
   "cell_type": "markdown",
   "metadata": {},
   "source": [
    "## Exponential time differencing methods (ETD)\n",
    "\n",
    "In the same conditions as above, it is taken a general Taylor expansion of $g$:\n",
    "\n",
    "$\\tau \\in (t_k, t_{k+1}), n \\in \\mathbb{N}$\n",
    "\n",
    "$$\n",
    "    g(y(\\tau), \\tau) = g(y(t_k), t_k) + (\\tau - t_k) \\frac{dg}{dt} (y(t_k), t_k) + \\frac{(\\tau - t_k)^2}{2!} \\frac{d^2g}{dt^2} (y(t_k), t_k) + \\\\\n",
    "    \\dotsi + \\frac{(\\tau - t_k)^{n-1}}{(n-1)!} \\frac{d^{n-1}g}{dt^{n-1}} (y(t_k), t_k) + \\frac{(\\tau - t_k)^n}{n!} \\frac{d^ng}{dt^n} (y(\\theta_k), \\theta_k)\n",
    "$$\n",
    "\n",
    "for a $\\theta_k \\in (t_k, t_{k+1})$\n",
    "\n",
    "In\n",
    "\n",
    "$$\n",
    "    y(t_{k+1}) = e^{-h \\lambda}y(t_k) + \\int_{t_k}^{t_{k+1}} e^{-\\lambda(t_{k+1}-\\tau)} g(y(\\tau), \\tau) d\\tau\n",
    "$$\n",
    "\n",
    "It will now become\n",
    "\n",
    "$$\n",
    "y(t_{k+1}) = e^{-h \\lambda}y(t_k) + \\int_{t_k}^{t_{k+1}} e^{-\\lambda(t_{k+1}-\\tau)}  g(y(t_k), t_k) +\n",
    "(\\tau - t_k) \\frac{dg}{dt} (y(t_k), t_k) +\n",
    "$$\n",
    "\n",
    "$$\n",
    " \\frac{(\\tau - t_k)^2}{2!} \\frac{d^2g}{dt^2} (y(t_k), t_k) + \\dotsi + \n",
    "$$\n",
    "\n",
    "$$\n",
    " + \\frac{(\\tau - t_k)^{n-1}}{(n-1)!} \\frac{d^{n-1}g}{dt^{n-1}} (y(t_k), t_k) + \\frac{(\\tau - t_k)^n}{n!} \\frac{d^ng}{dt^n} (y(\\theta_k), \\theta_k)  d\\tau,\n",
    "$$\n",
    "\n",
    "$$\n",
    "y(t_{k+1}) = e^{-h \\lambda}y(t_k) +\n",
    "g(y(t_k), t_k)\\int_{t_k}^{t_{k+1}} e^{-\\lambda(t_{k+1}-\\tau)} d \\tau +\n",
    "$$\n",
    "\n",
    "$$\n",
    "+ \\frac{dg}{dt}(y(t_k), t_k)\\int_{t_k}^{t_{k+1}} e^{-\\lambda(t_{k+1}-\\tau)} (\\tau - t_k)d\\tau + \\frac{d^2g}{dt^2} (y(t_k), t_k)\\int_{t_k}^{t_{k+1}} e^{-\\lambda(t_{k+1}-\\tau)} \\frac{(\\tau - t_k)^2}{2!}d\\tau +\n",
    "$$\n",
    "\n",
    "$$\n",
    "+ \\dotsi +\n",
    "$$\n",
    "\n",
    "$$\n",
    "+ \\frac{d^{n-1}g}{dt^{n-1}} (y(t_k), t_k)\\int_{t_k}^{t_{k+1}}  e^{-\\lambda(t_{k+1}-\\tau)} \\frac{(\\tau - t_k)^{n-1}}{(n-1)!} d\\tau + \\frac{d^ng}{dt^n} (y(\\theta_k), \\theta_k) \\int_{t_k}^{t_{k+1}}  e^{-\\lambda(t_{k+1}-\\tau)} \\frac{(\\tau - t_k)^n}{n!} d\\tau,\n",
    "$$\n",
    "\n",
    "$$\n",
    "y(t_{k+1}) = e^{-h \\lambda}y(t_k) +\n",
    "h\\phi_1(-\\lambda h) g(y(t_k), t_k) +\n",
    "h^2\\phi_2(-\\lambda h) \\frac{dg}{dt}(y(t_k), t_k) +\n",
    "h^3\\phi_3(-\\lambda h)\\frac{d^2g}{dt^2} (y(t_k), t_k)\n",
    "$$\n",
    "\n",
    "$$\n",
    "+ \\dotsi +\n",
    "$$\n",
    "\n",
    "$$\n",
    "+ h^n\\phi_n(-\\lambda h) \\frac{d^{n-1}g}{dt^{n-1}} (y(t_k), t_k)+\n",
    "h^{n+1}\\phi_{n+1}(-\\lambda h) \\frac{d^ng}{dt^n} (y(\\theta_k), \\theta_k).\n",
    "$$\n",
    "\n",
    "From the discussion about the exponential Euler, that is known that\n",
    "\n",
    "$$\n",
    "h^2\\phi_2(-\\lambda h) = \\frac{h^2}{2} - \\frac{h^3}{3!} \\lambda + \\dotsi + \\frac{h^l}{l!} (-\\lambda)^{l-2} + \\dotsi = \\frac{1}{(-\\lambda)^2} \\sum\\limits_{i=2}^{\\infty} \\frac{(-\\lambda h)^i}{i!}.\n",
    "$$\n",
    "\n",
    "Since\n",
    "\n",
    "$$\n",
    "  \\phi_{n+1}(-\\lambda h) = \\frac{\\phi_n(-\\lambda h) - \\phi_n(0)}{-\\lambda h} \\text{ and}\\\\\n",
    "  \\phi_n(0) = \\frac{1}{n!},\n",
    "$$\n",
    "\n",
    "$$\n",
    "  h^3 \\phi_3(-\\lambda h) = h^2 \\frac{\\phi_2(0) - \\phi_2(-\\lambda h)}{\\lambda} = \\frac{\\frac{h^2}{2} - (\\frac{h^2}{2} - \\frac{h^3}{3!} \\lambda + \\dotsi + \\frac{h^l}{l!} (-\\lambda)^{l-2} + O(h^{l+1}))}{\\lambda} = \\frac{1}{(-\\lambda)^3} \\sum\\limits_{i=3}^{\\infty} \\frac{(-\\lambda h)^i}{i!}.\n",
    "$$\n",
    "\n",
    "And if\n",
    "\n",
    "$$\n",
    "h^l \\phi_l(-\\lambda h) = \\frac{1}{(-\\lambda)^l} \\sum\\limits_{i=l}^{\\infty} \\frac{(-\\lambda h)^i}{i!}, \\text{for a } l \\in \\mathbb{N},\n",
    "$$\n",
    "\n",
    "$$\n",
    "  h^{l+1}\\phi_{l+1}(-\\lambda h) = h^{l+1} \\frac{\\phi_l(-\\lambda h) - \\phi_l(0)}{-\\lambda h} = \\frac{h^l \\phi_l(0) - h^l \\phi_l(-\\lambda h)}{\\lambda} = \\frac{h^l}{l! \\lambda} - \\frac{1}{\\lambda} \\frac{1}{(-\\lambda)^l} \\sum\\limits_{i=l}^{\\infty} \\frac{(-\\lambda h)^i}{i!} = \\frac{1}{(-\\lambda)^{l+1}} \\sum\\limits_{i=l+1}^{\\infty} \\frac{(-\\lambda h)^i}{i!}.\n",
    "$$\n",
    "\n",
    "So, by induction,\n",
    "\n",
    "$$\n",
    "h^n \\phi_n(-\\lambda h) = \\frac{1}{(-\\lambda)^n} \\sum\\limits_{i=n}^{\\infty} \\frac{(-\\lambda h)^i}{i!} = O(h^n), \\forall n \\geq 2.\n",
    "$$\n",
    "\n",
    "Then,\n",
    "\n",
    "$$\n",
    "y(t_{k+1}) = e^{-h \\lambda}y(t_k) +\n",
    "h\\phi_1(-\\lambda h) g(y(t_k), t_k) +\n",
    "h^2\\phi_2(-\\lambda h) \\frac{dg}{dt}(y(t_k), t_k) +\n",
    "h^3\\phi_3(-\\lambda h)\\frac{d^2g}{dt^2} (y(t_k), t_k) +\n",
    "\\dotsi + \\\\\n",
    "h^n\\phi_n(-\\lambda h) \\frac{d^{n-1}g}{dt^{n-1}} (y(t_k), t_k)+\n",
    "O(h^{n+1}).\n",
    "$$"
   ]
  },
  {
   "cell_type": "markdown",
   "metadata": {},
   "source": [
    "## Exponential time differencing methods with Runge-Kutta time stepping (ETDRK)\n",
    "\n",
    "For the Runge-Kutte methods, that is used approximations of the derivatives that converges together with the whole expression as the time step decreases.\n",
    "\n",
    "Before introducing the methods, the formatting of Butcher tableaus for ETDRK methods is shown."
   ]
  },
  {
   "cell_type": "markdown",
   "metadata": {},
   "source": [
    "### Butcher tableau for ETDRK\n",
    "\n",
    "The expressions of the ETDRK methods shown here are in the following format, being $s$ the order of the method,\n",
    "\n",
    "$$\n",
    "y(t_{k+1}) = e^{-h \\lambda} y(t_k) + h \\sum_{i = 1}^s b_i g\\left( t_k + c_i h, U_{ni} \\right),\n",
    "\\\\\n",
    "U_{ni} = e^{-c_i h \\lambda} y(t_k) + h \\sum_{j = 1}^s a_{ij} g\\left( t_k + c_j h, U_{nj} \\right),\n",
    "$$\n",
    "\n",
    "and its Butcher tableau is\n",
    "\n",
    "\\begin{array}\n",
    "{c|cccc}\n",
    "c_1 \\\\\n",
    "c_2 & a_{21} \\\\\n",
    "\\vdots & \\vdots & \\ddots \\\\\n",
    "c_s & a_{s1} & \\cdots & a_{s s-1}\\\\\n",
    "\\hline\n",
    "& b_1 & \\cdots & b_{s-1} & b_s \\text{   }.\n",
    "\\end{array}\n",
    "\n",
    "Based on [1]."
   ]
  },
  {
   "attachments": {},
   "cell_type": "markdown",
   "metadata": {},
   "source": [
    "### Order 2 - Trapezoidal rule\n",
    "\n",
    "For the second order method, that is used the approximation\n",
    "\n",
    "$$\n",
    "    g(y(\\tau), \\tau) = g(y(t_k), t_k) + (\\tau - t_k) \\frac{dg}{dt} (y(t_k), t_k) + O(h^2),\n",
    "$$\n",
    "\n",
    "$\\forall \\tau \\in (t_k, t_{k+1}).$\n",
    "\n",
    "The first derivative is discretized with the Taylor expansion\n",
    "\n",
    "$$\n",
    "g(y(t_{k+1}), t_{k+1}) = g(y(t_k), t_k) + h \\frac{dg}{dt} (y(t_k), t_k) + O(h^2)\n",
    "$$\n",
    "\n",
    "and the exponential Euler expression\n",
    "\n",
    "$$\n",
    "  y(t_{k+1}) = e^{-h \\lambda}y(t_k) + g(y(t_k), t_k) \\frac{1-e^{-h \\lambda}}{\\lambda} + O(h^2),\n",
    "$$\n",
    "\n",
    "so that\n",
    "\n",
    "$$\n",
    "\\frac{dg}{dt} (y(t_k), t_k)  = \\frac{g(a_k, t_{k+1}) - g(y(t_k), t_k)}{h} + O(h), \\\\\n",
    "\\text{with } a_k = e^{-h \\lambda}y(t_k) + g(y(t_k), t_k) \\frac{1-e^{-h\\lambda}}{\\lambda},\n",
    "$$\n",
    "\n",
    "which results in the expression\n",
    "\n",
    "$$\n",
    "g(y(\\tau), \\tau) = g(y(t_k), t_k) + (\\tau - t_k) \\frac{g(a_k, t_{k+1}) - g(y(t_k), t_k)}{h} + (\\tau - t_k)O(h) \\\\\n",
    "\\text{with } a_k = e^{-h \\lambda}y(t_k) + g(y(t_k), t_k) \\frac{1-e^{-h\\lambda}}{\\lambda}.\n",
    "$$\n",
    "\n",
    "Putting in the variation of constants formula\n",
    "\n",
    "$$\n",
    "y(t) = e^{-(t-t_0) \\lambda}y_0 + \\int_{t_0}^t e^{-\\lambda(t-\\tau)} g(y(\\tau), \\tau) d\\tau,\n",
    "$$\n",
    "\n",
    "$$\n",
    "  y(t_{k+1}) = e^{-h \\lambda}y(t_k) + \\\\\n",
    "  + \\int_{t_k}^{t_{k+1}} e^{-\\lambda(t_{k+1}-\\tau)} \\left[ g(y(t_k), t_k) + (\\tau - t_k)  \\frac{g(a_k, t_{k+1}) - g(y(t_k), t_k)}{h}  + (\\tau - t_k)O(h) \\right] d\\tau\n",
    "$$\n",
    "\n",
    "$$\n",
    "y(t_{k+1}) = e^{-h \\lambda} y(t_k) + g(y(t_k), t_k)\\int_{t_k}^{t_{k+1}} e^{-\\lambda(t_{k+1}-\\tau)} d \\tau + \\frac{g(a_k, t_{k+1}) - g(y(t_k), t_k)}{h} \\int_{t_k}^{t_{k+1}} (\\tau - t_k) e^{-\\lambda(t_{k+1}-\\tau)} d \\tau + \\\\\n",
    "+ O(h)\\int_{t_k}^{t_{k+1}} (\\tau - t_k) e^{-\\lambda(t_{k+1}-\\tau)} d \\tau \\\\\n",
    "\\text{with } a_k = e^{-h \\lambda}y(t_k) + g(y(t_k), t_k) \\frac{1-e^{-h\\lambda}}{\\lambda}.\n",
    "$$\n",
    "\n",
    "Then,\n",
    "\n",
    "$$\n",
    "y(t_{k+1}) = e^{-h \\lambda} y(t_k) +\n",
    "  h \\phi_1 (-\\lambda h) g(y(t_k), t_k) +\n",
    "  \\frac{g(a_k, t_{k+1}) - g(y(t_k), t_k)}{h} h^2 \\phi_2 (-\\lambda h) + \\\\\n",
    "  + O(h)h^2 \\phi_2 (-\\lambda h) \\\\\n",
    "  y(t_{k+1}) = e^{-h \\lambda} y(t_k) +\n",
    "  h \\phi_1 (-\\lambda h) g(y(t_k), t_k) +\n",
    "  \\left[g(a_k, t_{k+1}) - g(y(t_k), t_k) \\right] h \\phi_2 (-\\lambda h) + \\\\\n",
    "  + O(h^3) \\\\\n",
    "  \\text{with } a_k = e^{-h \\lambda}y(t_k) + g(y(t_k), t_k) \\frac{1-e^{-h\\lambda}}{\\lambda}.\n",
    "$$\n",
    "\n",
    "Butcher tableau:\n",
    "\n",
    "$$\n",
    "\\begin{array}\n",
    "{c|cc}\n",
    "0\\\\\n",
    "1 & \\phi_1(-\\lambda h)\\\\\n",
    "\\hline\n",
    "& \\phi_1 (-\\lambda h) - \\phi_2 (-\\lambda h) & \\phi_2 (-\\lambda h)\n",
    "\\end{array}\n",
    "$$"
   ]
  },
  {
   "attachments": {},
   "cell_type": "markdown",
   "metadata": {},
   "source": [
    "### Order 2 - Midpoint rule\n",
    "\n",
    "From the same expression:\n",
    "\n",
    "$$\n",
    "    g(y(\\tau), \\tau) = g(y(t_k), t_k) + (\\tau - t_k) \\frac{dg}{dt} (y(t_k), t_k) + O(h^2),\n",
    "$$\n",
    "\n",
    "$\\forall \\tau \\in (t_k, t_{k+1}).$\n",
    "\n",
    "The first derivative is now discretized with the Taylor expansion\n",
    "\n",
    "$$\n",
    "g\\left(y\\left(t_k + \\frac{h}{2}\\right), t_k + \\frac{h}{2} \\right) = g(y(t_k), t_k) + \\frac{h}{2} \\frac{dg}{dt} (y(t_k), t_k) + O(h^2)\n",
    "$$\n",
    "\n",
    "and the exponential Euler expression taken is with time step $\\frac{h}{2}$\n",
    " \n",
    "$$\n",
    "  y\\left(t_k + \\frac{h}{2}\\right) = e^{-\\frac{h \\lambda}{2}}y(t_k) + g(y(t_k), t_k) \\frac{h}{2} \\phi_1\\left( -\\frac{\\lambda h}{2} \\right) + O(h^2),\n",
    "$$\n",
    "\n",
    "so that\n",
    "\n",
    "$$\n",
    "\\frac{dg}{dt} (y(t_k), t_k)  = 2 \\frac{g\\left(b_k, t_k + \\frac{h}{2} \\right) - g(y(t_k), t_k)}{h} + O(h), \\\\\n",
    "\\text{with } b_k =e^{-\\frac{h \\lambda}{2}}y(t_k) + g(y(t_k), t_k) \\frac{h}{2} \\phi_1\\left( -\\frac{\\lambda h}{2} \\right),\n",
    "$$\n",
    "\n",
    "which results in the expression\n",
    "\n",
    "$$\n",
    "g(y(\\tau), \\tau) = g(y(t_k), t_k) + 2(\\tau - t_k) \\frac{g\\left(b_k, t_k + \\frac{h}{2}\\right) - g(y(t_k), t_k)}{h} + (\\tau - t_k)O(h) \\\\\n",
    "\\text{with } b_k =e^{-\\frac{h \\lambda}{2}}y(t_k) + g(y(t_k), t_k) \\frac{h}{2} \\phi_1\\left( -\\frac{\\lambda h}{2} \\right).\n",
    "$$\n",
    "\n",
    "Putting in the variation of constants formula\n",
    "\n",
    "$$\n",
    "y(t) = e^{-(t-t_0) \\lambda}y_0 + \\int_{t_0}^t e^{-\\lambda(t-\\tau)} g(y(\\tau), \\tau) d\\tau,\n",
    "$$\n",
    "\n",
    "$$\n",
    "  y(t_{k+1}) = e^{-h \\lambda}y(t_k) + \\\\\n",
    "    + \\int_{t_k}^{t_{k+1}} e^{-\\lambda(t_{k+1}-\\tau)} \\left[ g(y(t_k), t_k) + 2(\\tau - t_k) \\frac{g\\left(b_k, t_k + \\frac{h}{2}\\right) - g(y(t_k), t_k)}{h} + (\\tau - t_k)O(h) \\right] d\\tau\n",
    "$$\n",
    "\n",
    "$$\n",
    "y(t_{k+1}) = e^{-h \\lambda} y(t_k) + g(y(t_k), t_k)\\int_{t_k}^{t_{k+1}} e^{-\\lambda(t_{k+1}-\\tau)} d \\tau + \\\\\n",
    "  + 2\\frac{g\\left(b_k, t_k + \\frac{h}{2}\\right) - g(y(t_k), t_k)}{h} \\int_{t_k}^{t_{k+1}} (\\tau - t_k) e^{-\\lambda(t_{k+1}-\\tau)} d \\tau + O(h)\\int_{t_k}^{t_{k+1}} (\\tau - t_k) e^{-\\lambda(t_{k+1}-\\tau)} d \\tau \\\\\n",
    "  \\text{with } b_k =e^{-\\frac{h \\lambda}{2}}y(t_k) + g(y(t_k), t_k) \\frac{h}{2} \\phi_1\\left( -\\frac{\\lambda h}{2} \\right).\n",
    "$$\n",
    "\n",
    "Then,\n",
    "\n",
    "$$\n",
    "y(t_{k+1}) = e^{-h \\lambda} y(t_k) +\n",
    "  h \\phi_1 (-\\lambda h) g(y(t_k), t_k) +\n",
    "  2\\frac{g\\left(b_k, t_k + \\frac{h}{2}\\right) - g(y(t_k), t_k)}{h} h^2 \\phi_2 (-\\lambda h) + \\\\\n",
    "  + O(h)h^2 \\phi_2 (-\\lambda h) \\\\\n",
    "  y(t_{k+1}) = e^{-h \\lambda} y(t_k) +\n",
    "  h \\phi_1 (-\\lambda h) g(y(t_k), t_k) +\n",
    "  2 \\left[g\\left(b_k, t_k + \\frac{h}{2}\\right) - g(y(t_k), t_k) \\right] h \\phi_2 (-\\lambda h) + \\\\\n",
    "  + O(h^3) \\\\\n",
    "  \\text{with } b_k =e^{-\\frac{h \\lambda}{2}}y(t_k) + g(y(t_k), t_k) \\frac{h}{2} \\phi_1\\left( -\\frac{\\lambda h}{2} \\right).\n",
    "$$\n",
    "\n",
    "Butcher tableau:\n",
    "\n",
    "\\begin{array}\n",
    "{c|cc}\n",
    "0\\\\\n",
    "\\frac{1}{2} & \\frac{1}{2}\\phi_1\\left(-\\frac{\\lambda h}{2}\\right)\\\\\n",
    "\\hline\n",
    "& \\phi_1 (-\\lambda h) - 2 \\phi_2 (-\\lambda h) & -2 \\phi_2 (-\\lambda h)\n",
    "\\end{array}"
   ]
  },
  {
   "attachments": {},
   "cell_type": "markdown",
   "metadata": {},
   "source": [
    "### Naive method - order 2 - Trapezoidal rule\n",
    "\n",
    "It is also possible to think the exponential time differencing methods with Runge-Kutta time stepping using the numerical integration, for example, for the one with second order, it starts with the trapezoidal rule (which was taken from [2]) on the variation of constants formula:\n",
    "\n",
    "$$\n",
    "y(t_{k+1}) = e^{-h \\lambda}y(t_k) + \\frac{h}{2} \\left[ e^{-\\lambda(t_{k+1}-t_k)} g(y(t_k), t_k) + e^{-\\lambda(t_{k+1}-t_{k+1})} g(y(t_{k+1}), t_{k+1}) \\right] + O(h^3), \\\\\n",
    "    y(t_{k+1}) = e^{-h \\lambda}y(t_k) + \\frac{h}{2} \\left[ e^{-\\lambda h} g(y(t_k), t_k) + g(y(t_{k+1}), t_{k+1}) \\right] +  O(h^3).\n",
    "$$\n",
    "\n",
    "And then, from the expression seen before:\n",
    "\n",
    "$$\n",
    "y(t_{k+1}) = e^{-h \\lambda}y(t_k) + g(y(t_k), t_k) \\frac{1-e^{-h \\lambda}}{\\lambda} + O(h^2),\n",
    "$$\n",
    "\n",
    "$$\n",
    "    g(y(t_{k+1}), t_{k+1}) = g(a_k, t_{k+1}) + O(h^2) \\text{, with } a_k = e^{-h \\lambda}y(t_k) + g(y(t_k), t_k) \\frac{1-e^{-h\\lambda}}{\\lambda}.\n",
    "$$\n",
    "\n",
    "So,\n",
    "\n",
    "$$\n",
    "y(t_{k+1}) = e^{-h \\lambda}y(t_k) + \\frac{h}{2} \\left[ e^{-\\lambda h} g(y(t_k), t_k) + g(a_k, t_{k+1}) + O(h^2) \\right] +  O(h^3),\n",
    "$$\n",
    "\n",
    "$$\n",
    "y(t_{k+1}) = e^{-h \\lambda}y(t_k) + \\frac{h}{2} \\left[ e^{-\\lambda h} g(y(t_k), t_k) + g(a_k, t_{k+1}) \\right] +  O(h^3) \\\\\n",
    "    \\text{with } a_k = e^{-h \\lambda}y(t_k) + g(y(t_k), t_k) h \\phi_1 (-\\lambda h).\n",
    "$$\n",
    "\n",
    "Butcher tableau:\n",
    "\n",
    "$$\n",
    "\\begin{array}\n",
    "{c|cc}\n",
    "0\\\\\n",
    "1 & \\phi_1(-\\lambda h)\\\\\n",
    "\\hline\n",
    "& \\frac{1}{2} e^{-h \\lambda} & \\frac{1}{2}\n",
    "\\end{array}\n",
    "$$"
   ]
  },
  {
   "attachments": {},
   "cell_type": "markdown",
   "metadata": {},
   "source": [
    "### Naive method - order 2 - Midpoint rule\n",
    "\n",
    "Besides that, using the midpoint rule, also known as rectangle rule, again taken from [2],\n",
    "\n",
    "$$\n",
    "y(t_{k+1}) = e^{-(t_{k+1}-t_k) \\lambda}y(t_k) + \\int_{t_k}^{t_{k+1}} [e^{-\\lambda(t_{k+1}-\\tau)} g(y(\\tau), \\tau)] d\\tau,\n",
    "$$\n",
    "\n",
    "$$\n",
    "y(t_{k+1}) = e^{-h\\lambda}y(t_k) + h e^{-\\lambda\\left(t_{k+1}-\\frac{t_{k+1}+t_k}{2}\\right)} g\\left(y\\left(\\frac{t_{k+1}+t_k}{2}\\right), \\frac{t_{k+1}+t_k}{2}\\right) + O(h^3),\n",
    "$$\n",
    "\n",
    "$$\n",
    "y(t_{k+1}) = e^{-h\\lambda}y(t_k) + h e^{- \\frac{h\\lambda}{2}} g\\left(y\\left(t_k + \\frac{h}{2}\\right), t_k+\\frac{h}{2}\\right) + O(h^3),\n",
    "$$\n",
    "\n",
    "and Exponential Euler with time step $\\frac{h}{2}$\n",
    "\n",
    "$$\n",
    "y\\left(t_k + \\frac{h}{2}\\right) = e^{-\\frac{h \\lambda}{2}}y(t_k) + g(y(t_k), t_k) \\frac{h}{2} \\phi_1\\left( -\\frac{\\lambda h}{2} \\right) + O(h^2),\n",
    "$$\n",
    "\n",
    "results in\n",
    "\n",
    "$$\n",
    "y(t_{k+1}) = e^{-h\\lambda}y(t_k) + h e^{- \\frac{h\\lambda}{2}} g\\left(b_k + O(h^2), t_k + \\frac{h}{2}\\right) + O(h^3) \\\\\n",
    "    \\text{with } b_k =e^{-\\frac{h \\lambda}{2}}y(t_k) + g(y(t_k), t_k) \\frac{h}{2} \\phi_1\\left( -\\frac{\\lambda h}{2} \\right),\n",
    "$$\n",
    "\n",
    "$$\n",
    "y(t_{k+1}) = e^{-h\\lambda}y(t_k) + h e^{- \\frac{h\\lambda}{2}} g\\left(b_k , t_k + \\frac{h}{2}\\right) + O(h^3) \\\\\n",
    "    \\text{with } b_k =e^{-\\frac{h \\lambda}{2}}y(t_k) + g(y(t_k), t_k) \\frac{h}{2} \\phi_1\\left( -\\frac{\\lambda h}{2} \\right),\n",
    "$$\n",
    "\n",
    "Butcher tableau:\n",
    "\n",
    "$$\n",
    "\\begin{array}\n",
    "{c|cc}\n",
    "0\\\\\n",
    "\\frac{1}{2} &  \\frac{1}{2} \\phi_1( -\\frac{\\lambda h}{2})\\\\\n",
    "\\hline\n",
    "& 0 & e^{-\\frac{h \\lambda}{2}}\n",
    "\\end{array}\n",
    "$$"
   ]
  },
  {
   "cell_type": "markdown",
   "metadata": {},
   "source": [
    "### Order 3 - similar\n",
    "\n",
    "$\\textbf{Note: }$ It is called similar because does not follows the format of Runge Kutta functions, with its Butcher tableau being triangular, but is indeed exponential.\n",
    "\n",
    "For the third order method, that is used the approximation\n",
    "\n",
    "$$\n",
    "    g(y(\\tau), \\tau) = g\\left(y\\left(t_{k+\\frac{1}{2}}\\right), t_{k+\\frac{1}{2}}\\right) +\n",
    "    \\left(\\tau - t_{k+\\frac{1}{2}}\\right) \\frac{dg}{dt} \\left(y\\left(t_{k+\\frac{1}{2}}\\right), t_{k+\\frac{1}{2}}\\right) + \\\\\n",
    "    + \\frac{\\left(\\tau - t_{k+\\frac{1}{2}}\\right)^2}{2!} \\frac{d^2g}{dt^2} \\left(y\\left(t_{k+\\frac{1}{2}}\\right), t_{k+\\frac{1}{2}}\\right) + \\\\\n",
    "    + \\frac{\\left(\\tau - t_{k+\\frac{1}{2}}\\right)^3}{3!} \\frac{d^3g}{dt^3} \\left(y\\left(t_{k+\\frac{1}{2}}\\right), t_{k+\\frac{1}{2}}\\right)\n",
    "    + O((\\tau - t_k)^4),\n",
    "$$\n",
    "\n",
    "$\\forall \\tau \\in \\mathbb{R}.$\n",
    "\n",
    "In order to approximate the derivatives, there is taken\n",
    "\n",
    "$$\n",
    "    g(y(t_{k+1}), t_{k+1}) = g\\left(y\\left(t_{k+\\frac{1}{2}}\\right), t_{k+\\frac{1}{2}}\\right) +\n",
    "    \\left(t_{k+1} - t_{k+\\frac{1}{2}}\\right) \\frac{dg}{dt} \\left(y\\left(t_{k+\\frac{1}{2}}\\right), t_{k+\\frac{1}{2}}\\right) + \\\\\n",
    "    + \\frac{\\left(t_{k+1} - t_{k+\\frac{1}{2}}\\right)^2}{2!} \\frac{d^2g}{dt^2} \\left(y\\left(t_{k+\\frac{1}{2}}\\right), t_{k+\\frac{1}{2}}\\right) + \\\\\n",
    "    + \\frac{\\left(t_{k+1} - t_{k+\\frac{1}{2}}\\right)^3}{3!} \\frac{d^3g}{dt^3} \\left(y\\left(t_{k+\\frac{1}{2}}\\right), t_{k+\\frac{1}{2}}\\right)\n",
    "    + O(h^4),\n",
    "$$\n",
    "\n",
    "$$\n",
    "    g(y(t_{k+1}), t_{k+1}) = g\\left(y\\left(t_{k+\\frac{1}{2}}\\right), t_{k+\\frac{1}{2}}\\right) +\n",
    "    \\frac{h}{2} \\frac{dg}{dt} \\left(y\\left(t_{k+\\frac{1}{2}}\\right), t_{k+\\frac{1}{2}}\\right) + \\\\\n",
    "    +\\frac{h^2}{8} \\frac{d^2g}{dt^2} \\left(y\\left(t_{k+\\frac{1}{2}}\\right), t_{k+\\frac{1}{2}}\\right)\n",
    "    + \\frac{h^3}{48} \\frac{d^3g}{dt^3} \\left(y\\left(t_{k+\\frac{1}{2}}\\right), t_{k+\\frac{1}{2}}\\right)\n",
    "    + O(h^4),\n",
    "$$\n",
    "\n",
    "and\n",
    "\n",
    "$$\n",
    "    g(y(t_k), t_k) = g\\left(y\\left(t_{k+\\frac{1}{2}}\\right), t_{k+\\frac{1}{2}}\\right) +\n",
    "    \\left(t_k - t_{k+\\frac{1}{2}}\\right) \\frac{dg}{dt} \\left(y\\left(t_{k+\\frac{1}{2}}\\right), t_{k+\\frac{1}{2}}\\right) + \\\\\n",
    "    + \\frac{\\left(t_k - t_{k+\\frac{1}{2}}\\right)^2}{2!} \\frac{d^2g}{dt^2} \\left(y\\left(t_{k+\\frac{1}{2}}\\right), t_{k+\\frac{1}{2}}\\right) + \\\\\n",
    "    + \\frac{\\left(t_k - t_{k+\\frac{1}{2}}\\right)^3}{3!} \\frac{d^3g}{dt^3} \\left(y\\left(t_{k+\\frac{1}{2}}\\right), t_{k+\\frac{1}{2}}\\right)\n",
    "    + O(h^4),\n",
    "$$\n",
    "\n",
    "$$\n",
    "    g(y(t_k), t_k) = g\\left(y\\left(t_{k+\\frac{1}{2}}\\right), t_{k+\\frac{1}{2}}\\right) -\n",
    "    \\frac{h}{2} \\frac{dg}{dt} \\left(y\\left(t_{k+\\frac{1}{2}}\\right), t_{k+\\frac{1}{2}}\\right) + \\\\\n",
    "    + \\frac{h^2}{8} \\frac{d^2g}{dt^2} \\left(y\\left(t_{k+\\frac{1}{2}}\\right), t_{k+\\frac{1}{2}}\\right)\n",
    "    - \\frac{h^3}{48} \\frac{d^3g}{dt^3} \\left(y\\left(t_{k+\\frac{1}{2}}\\right), t_{k+\\frac{1}{2}}\\right)\n",
    "    + O(h^4).\n",
    "$$\n",
    "\n",
    "Subtracting the two expressions,\n",
    "\n",
    "$$\n",
    "  g(y(t_{k+1}), t_{k+1}) - g(y(t_k), t_k) = h \\frac{dg}{dt} \\left(y\\left(t_{k+\\frac{1}{2}}\\right), t_{k+\\frac{1}{2}}\\right) + O(h^3).\n",
    "$$\n",
    "\n",
    "So,\n",
    "\n",
    "$$\n",
    "  \\frac{dg}{dt} \\left(y\\left(t_{k+\\frac{1}{2}}\\right), t_{k+\\frac{1}{2}}\\right) = \\frac{g(y(t_{k+1}), t_{k+1}) - g(y(t_k), t_k)}{h} + O(h^2).\n",
    "$$\n",
    "\n",
    "And summing them\n",
    "\n",
    "$$\n",
    "  g(y(t_{k+1}), t_{k+1}) + g(y(t_k), t_k) =\n",
    "  2 g\\left(y\\left(t_{k+\\frac{1}{2}}\\right), t_{k+\\frac{1}{2}}\\right)\n",
    "  + \\frac{h^2}{4} \\frac{d^2g}{dt^2} \\left(y\\left(t_{k+\\frac{1}{2}}\\right), t_{k+\\frac{1}{2}}\\right) + O(h^4).\n",
    "$$\n",
    "\n",
    "This results in the expression\n",
    "\n",
    "$$\n",
    "    g(y(\\tau), \\tau) = g\\left(y\\left(t_{k+\\frac{1}{2}}\\right), t_{k+\\frac{1}{2}}\\right) +\n",
    "    \\left(\\tau - t_{k+\\frac{1}{2}}\\right)  \\frac{g(y(t_{k+1}), t_{k+1}) - g(y(t_k), t_k)}{h} + \\\\\n",
    "    + \\frac{\\left(\\tau - t_{k+\\frac{1}{2}}\\right)^2}{2!} \\frac{ 4 \\left[g(y(t_{k+1}), t_{k+1}) + g(y(t_k), t_k) -\n",
    "  2 g\\left(y\\left(t_{k+\\frac{1}{2}}\\right), t_{k+\\frac{1}{2}}\\right) \\right]}{h^2} + \\\\\n",
    "    + O((\\tau - t_k)^3),\n",
    "$$\n",
    "\n",
    "$\\forall \\tau \\in \\mathbb{R}.$\n",
    "\n",
    "Putting in the variation of constants formula\n",
    "\n",
    "$$\n",
    "y(t) = e^{-(t-t_0) \\lambda}y_0 + \\int_{t_0}^t e^{-\\lambda(t-\\tau)} g(y(\\tau), \\tau) d\\tau,\n",
    "$$\n",
    "\n",
    "$$\n",
    "  y(t_{k+1}) = e^{-h \\lambda}y(t_k) + \\\\\n",
    "  + \\int_{t_k}^{t_{k+1}} e^{-\\lambda(t_{k+1}-\\tau)} \\left[ g\\left(y\\left(t_{k+\\frac{1}{2}}\\right), t_{k+\\frac{1}{2}}\\right) +\n",
    "    \\left(\\tau - t_{k+\\frac{1}{2}}\\right)  \\frac{g(y(t_{k+1}), t_{k+1}) - g(y(t_k), t_k)}{h} + \\\\\n",
    "    + \\frac{\\left(\\tau - t_{k+\\frac{1}{2}}\\right)^2}{2!} \\frac{ 4 \\left[g(y(t_{k+1}), t_{k+1}) + g(y(t_k), t_k) -\n",
    "  2 g\\left(y\\left(t_{k+\\frac{1}{2}}\\right), t_{k+\\frac{1}{2}}\\right) \\right]}{h^2} + O((\\tau - t_k)^3) \\right] d\\tau,\n",
    "$$\n",
    "\n",
    "$$\n",
    "  y(t_{k+1}) = e^{-h \\lambda} y(t_k) +\n",
    "  g\\left(y\\left(t_{k+\\frac{1}{2}}\\right), t_{k+\\frac{1}{2}}\\right)\n",
    "  \\int_{t_k}^{t_{k+1}} e^{-\\lambda(t_{k+1}-\\tau)} d \\tau +\n",
    "  \\frac{g(y(t_{k+1}), t_{k+1}) - g(y(t_k), t_k)}{h}\n",
    "  \\int_{t_k}^{t_{k+1}} \\left(\\tau - t_{k+\\frac{1}{2}}\\right) e^{-\\lambda(t_{k+1}-\\tau)} d \\tau +\n",
    "  \\\\\n",
    "  + \\frac{ 4 \\left[g(y(t_{k+1}), t_{k+1}) + g(y(t_k), t_k) - 2 g\\left(y\\left(t_{k+\\frac{1}{2}}\\right), t_{k+\\frac{1}{2}}\\right) \\right]}{h^2}\n",
    "  \\int_{t_k}^{t_{k+1}} \\frac{\\left(\\tau - t_{k+\\frac{1}{2}}\\right)^2}{2!} e^{-\\lambda(t_{k+1}-\\tau)} d \\tau\n",
    "  + \\int_{t_k}^{t_{k+1}} O((\\tau - t_k)^3) e^{-\\lambda(t_{k+1}-\\tau)} d \\tau,\n",
    "$$\n",
    "\n",
    "Since $\\tau - t_{k+ \\frac{1}{2}} = \\tau - t_k - \\frac{h}{2}$ and $\\left(\\tau - t_{k+ \\frac{1}{2}} \\right)^2 = (\\tau - t_k)^2 + \\frac{h^2}{4} - h (\\tau - t_k)$,\n",
    "\n",
    "$$\n",
    "  y(t_{k+1}) = e^{-h \\lambda} y(t_k) +\n",
    "  g\\left(y\\left(t_{k+\\frac{1}{2}}\\right), t_{k+\\frac{1}{2}}\\right)\n",
    "  \\int_{t_k}^{t_{k+1}} e^{-\\lambda(t_{k+1}-\\tau)} d \\tau +\n",
    "  \\frac{g(y(t_{k+1}), t_{k+1}) - g(y(t_k), t_k)}{h}\n",
    "  \\int_{t_k}^{t_{k+1}} \\left(\\tau - t_{k}\\right) e^{-\\lambda(t_{k+1}-\\tau)} d \\tau +\n",
    "  \\\\\n",
    "  + \\frac{ 4 \\left[g(y(t_{k+1}), t_{k+1}) + g(y(t_k), t_k) - 2 g\\left(y\\left(t_{k+\\frac{1}{2}}\\right), t_{k+\\frac{1}{2}}\\right) \\right]}{h^2}\n",
    "  \\int_{t_k}^{t_{k+1}} \\frac{(\\tau - t_k)^2}{2!} e^{-\\lambda(t_{k+1}-\\tau)} d \\tau +\n",
    "  \\\\\n",
    "  - \\frac{g(y(t_{k+1}), t_{k+1}) - g(y(t_k), t_k)}{h}\n",
    "  \\int_{t_k}^{t_{k+1}} \\frac{h}{2} e^{-\\lambda(t_{k+1}-\\tau)} d \\tau +\n",
    "  \\\\\n",
    "  + \\frac{ 4 \\left[g(y(t_{k+1}), t_{k+1}) + g(y(t_k), t_k) - 2 g\\left(y\\left(t_{k+\\frac{1}{2}}\\right), t_{k+\\frac{1}{2}}\\right) \\right]}{h^2}\n",
    "  \\int_{t_k}^{t_{k+1}} \\frac{h^2}{4 \\cdot 2!} e^{-\\lambda(t_{k+1}-\\tau)} d \\tau +\n",
    "  \\\\\n",
    "  - \\frac{ 4 \\left[g(y(t_{k+1}), t_{k+1}) + g(y(t_k), t_k) - 2 g\\left(y\\left(t_{k+\\frac{1}{2}}\\right), t_{k+\\frac{1}{2}}\\right) \\right]}{h^2}\n",
    "  \\int_{t_k}^{t_{k+1}} \\frac{h (\\tau - t_k)}{2!} e^{-\\lambda(t_{k+1}-\\tau)} d \\tau +\n",
    "  \\\\\n",
    "  + \\int_{t_k}^{t_{k+1}} O((\\tau - t_k)^3) e^{-\\lambda(t_{k+1}-\\tau)} d \\tau.\n",
    "$$\n",
    "\n",
    "Then,\n",
    "\n",
    "$$\n",
    "  y(t_{k+1}) = e^{-h \\lambda} y(t_k) +\n",
    "  g\\left(y\\left(t_{k+\\frac{1}{2}}\\right), t_{k+\\frac{1}{2}}\\right)\n",
    "  h \\phi_1(-h \\lambda) +\n",
    "  \\frac{g(y(t_{k+1}), t_{k+1}) - g(y(t_k), t_k)}{h}\n",
    "  h^2 \\phi_2 (-h \\lambda) +\n",
    "  \\\\\n",
    "  + \\frac{ 4 \\left[g(y(t_{k+1}), t_{k+1}) + g(y(t_k), t_k) - 2 g\\left(y\\left(t_{k+\\frac{1}{2}}\\right), t_{k+\\frac{1}{2}}\\right) \\right]}{h^2}\n",
    "  h^3 \\phi_3 (-h \\lambda) +\n",
    "  \\\\\n",
    "  - \\frac{g(y(t_{k+1}), t_{k+1}) - g(y(t_k), t_k)}{h}\n",
    "  \\frac{h^2 \\phi_1(-h \\lambda)}{2} +\n",
    "  \\\\\n",
    "  + \\frac{ 4 \\left[g(y(t_{k+1}), t_{k+1}) + g(y(t_k), t_k) - 2 g\\left(y\\left(t_{k+\\frac{1}{2}}\\right), t_{k+\\frac{1}{2}}\\right) \\right]}{h^2}\n",
    "  \\frac{h^3 \\phi_1(-h \\lambda)}{8} +\n",
    "  \\\\\n",
    "  - \\frac{ 4 \\left[g(y(t_{k+1}), t_{k+1}) + g(y(t_k), t_k) - 2 g\\left(y\\left(t_{k+\\frac{1}{2}}\\right), t_{k+\\frac{1}{2}}\\right) \\right]}{h^2}\n",
    "  \\frac{h^3 \\phi_2(-h \\lambda)}{2} +\n",
    "  \\\\\n",
    "  + O(h^4 \\phi_4(-h \\lambda)).\n",
    "$$\n",
    "\n",
    "i.e.\n",
    "\n",
    "$$\n",
    "  y(t_{k+1}) = e^{-h \\lambda} y(t_k) +\n",
    "  g\\left(y\\left(t_{k+\\frac{1}{2}}\\right), t_{k+\\frac{1}{2}}\\right)\n",
    "  h \\phi_1(-h \\lambda) + %ok\n",
    "  \\left[g(y(t_{k+1}), t_{k+1}) - g(y(t_k), t_k)\\right]\n",
    "  \\left( h \\phi_2 (-h \\lambda) - \\frac{h \\phi_1(-h \\lambda)}{2} \\right) +\n",
    "  \\\\\n",
    "  + 4 \\left[g(y(t_{k+1}), t_{k+1}) + g(y(t_k), t_k) - 2 g\\left(y\\left(t_{k+\\frac{1}{2}}\\right), t_{k+\\frac{1}{2}}\\right) \\right]\n",
    "  \\left( h \\phi_3 (-h \\lambda) + \\frac{h \\phi_1(-h \\lambda)}{8} - \\frac{h \\phi_2(-h \\lambda)}{2} \\right) + O(h^4).\n",
    "$$\n",
    "\n",
    "Using the ETD2RK expressions (trapezoid) to approximate $y\\left(t_{k+\\frac{1}{2}}\\right)$ and $y(t_{k+1})$, since those are of order 2, i.e., $O(h^3)$, the expression of the method is\n",
    "\n",
    "$$\n",
    "  y(t_{k+1}) = e^{-h \\lambda} y(t_k) +\n",
    "  g\\left(c'_k, t_{k+\\frac{1}{2}}\\right)\n",
    "  h \\phi_1(-h \\lambda) + %ok\n",
    "  \\left[g(c_k, t_{k+1}) - g(y(t_k), t_k)\\right]\n",
    "  \\left( h \\phi_2 (-h \\lambda) - \\frac{h \\phi_1(-h \\lambda)}{2} \\right) +\n",
    "  \\\\\n",
    "  + 4 \\left[g(c_k, t_{k+1}) + g(y(t_k), t_k) - 2 g\\left(c'_k, t_{k+\\frac{1}{2}}\\right) \\right]\n",
    "  \\left( h \\phi_3 (-h \\lambda) + \\frac{h \\phi_1(-h \\lambda)}{8} - \\frac{h \\phi_2(-h \\lambda)}{2} \\right) + O(h^4),\n",
    "$$\n",
    "\n",
    "with\n",
    "\n",
    "$$\n",
    "  c_k = e^{-h \\lambda} y(t_k) +\n",
    "  h \\phi_1 (-\\lambda h) g(y(t_k), t_k) +\n",
    "  \\left[g(a_k, t_{k+1}) - g(y(t_k), t_k) \\right] h \\phi_2 (-\\lambda h),\n",
    "  \\\\\n",
    "  a_k = e^{-h \\lambda}y(t_k) + g(y(t_k), t_k) h \\phi_1(-h\\lambda),\n",
    "  \\\\\n",
    "  c'_k = e^{- \\frac{h \\lambda}{2}} y(t_k) +\n",
    "  \\frac{h}{2} \\phi_1 \\left(- \\frac{\\lambda h}{2} \\right) g(y(t_k), t_k) +\n",
    "  \\left[g\\left(a'_k, t_{k+\\frac{1}{2}}\\right) - g(y(t_k), t_k) \\right] \\frac{h}{2} \\phi_2 \\left(-\\frac{\\lambda h}{2}\\right),\n",
    "  \\\\\n",
    "  a'_k = e^{-\\frac{h \\lambda}{2}}y(t_k) + g(y(t_k), t_k) \\frac{h}{2} \\phi_1\\left(-\\frac{h \\lambda}{2}\\right).\n",
    "$$\n",
    "\n",
    "As said earlier, the Butcher tableau doesn't work here because this method does not follows the RK format, the following tableau isn't showing all the information about the method but ilustrates in part how it is:\n",
    "\n",
    "\\begin{array}\n",
    "{c|cccc}\n",
    "0 \\\\\n",
    "\\frac{1}{2} & \\frac{1}{2} \\left( \\phi_1\\left(- \\frac{\\lambda h}{2} \\right) - \\phi_2\\left(- \\frac{\\lambda h}{2} \\right) \\right) & \\frac{1}{2}\\phi_2\\left(- \\frac{\\lambda h}{2} \\right) \\\\\n",
    "1 & \\phi_1\\left(- \\lambda h \\right) - \\phi_2\\left(- \\lambda h \\right) & 0 & \\phi_2\\left(- \\lambda h \\right)  \\\\\n",
    "\\hline\n",
    "& 4 \\phi_3(-h \\lambda)-3\\phi_2(-h\\lambda)+\\phi_1(-h\\lambda) & -8\\phi_3(-h\\lambda)+4\\phi_2(-h\\lambda) & 4 \\phi_3(-h\\lambda)-\\phi_2(-h\\lambda) \\text{   }.\n",
    "\\end{array}"
   ]
  },
  {
   "cell_type": "markdown",
   "metadata": {},
   "source": [
    "### Naive method - Order 3\n",
    "\n",
    "Here, that is taken the variation of constants formula:\n",
    "\n",
    "$$\n",
    "    y(t_{k+1}) = e^{-h \\lambda}y(t_k) + \\int_{t_k}^{t_{k+1}} e^{-\\lambda(t_{k+1}-\\tau)} g(y(\\tau), \\tau) d\\tau,\n",
    "$$\n",
    "\n",
    "and applied the Simpson's rule (here was used the order of convergence from Burden) so that it will be:\n",
    "\n",
    "$$\n",
    "    y(t_{k+1}) = e^{-h \\lambda}y(t_k) + \\frac{h}{6} \\left[ e^{-\\lambda(t_{k+1}-t_k)} g(y(t_k), t_k) + 4 e^{-\\lambda \\left(t_{k+1}-t_{k + \\frac{1}{2}} \\right)} g\\left(y\\left(t_{k+\\frac{1}{2}}\\right), t_k + \\frac{h}{2} \\right) \\\\ + e^{-\\lambda(t_{k+1}-t_{k+1})} g(y(t_{k+1}), t_{k+1}) \\right] + O(h^5), \\\\\n",
    "    y(t_{k+1}) = e^{-h \\lambda}y(t_k) + \\frac{h}{6} \\left[ e^{-\\lambda h} g(y(t_k), t_k) + 4 e^{-\\frac{ \\lambda h}{2}} g\\left(y\\left(t_k + \\frac{h}{2} \\right), t_k + \\frac{h}{2} \\right) + g(y(t_{k+1}), t_{k+1}) \\right] +  O(h^5).\n",
    "$$\n",
    "\n",
    "To approximate $y\\left(t_k + \\frac{h}{2} \\right)$:\n",
    "\n",
    "$$\n",
    "    y\\left(t_k + \\frac{h}{2} \\right) = e^{- \\frac{h \\lambda}{2}}y(t_k) + \\frac{h}{4} \\left[ e^{- \\frac{h \\lambda}{2}} g(y(t_k), t_k) + g \\left(a'_{k}, t_k + \\frac{h}{2} \\right) \\right] +  O(h^3), \\\\\n",
    "    \\text{with } a'_{k} = e^{- \\frac{h \\lambda}{2}} y(t_k) + g(y(t_k), t_k) \\frac{h}{2} \\phi_1 \\left(-\\lambda \\frac{h}{2} \\right),\n",
    "$$\n",
    "\n",
    "and, for $y\\left(t_{k+1} \\right)$:\n",
    "\n",
    "$$\n",
    "    y(t_{k+1}) = e^{-h \\lambda}y(t_k) + \\frac{h}{2} \\left[ e^{-\\lambda h} g(y(t_k), t_k) + g(a_k, t_{k+1}) \\right] +  O(h^3), \\\\\n",
    "    \\text{with } a_k = e^{-h \\lambda}y(t_k) + g(y(t_k), t_k) h \\phi_1 (-\\lambda h).\n",
    "$$\n",
    "\n",
    "So, the expression is\n",
    "\n",
    "$$\n",
    "  y(t_{k+1}) = e^{-h \\lambda}y(t_k) + \\frac{h}{6} \\left[ e^{-\\lambda h} g(y(t_k), t_k) + 4 e^{-\\frac{ \\lambda h}{2}} g\\left( b'_{k}, t_k + \\frac{h}{2} \\right) + g(b_k, t_{k+1}) \\right] +  O(h^4), \\\\\n",
    "  \\text{with } b'_{k} = e^{- \\frac{h \\lambda}{2}}y(t_k) + \\frac{h}{4} \\left[ e^{- \\frac{h \\lambda}{2}} g(y(t_k), t_k) + g \\left(a'_{k}, t_k + \\frac{h}{2} \\right) \\right], \\\\\n",
    "  b_k = e^{-h \\lambda}y(t_k) + \\frac{h}{2} \\left[ e^{-\\lambda h} g(y(t_k), t_k) + g(a_k, t_{k+1}) \\right], \\\\\n",
    "  a'_{k} = e^{- \\frac{h \\lambda}{2}} y(t_k) + g(y(t_k), t_k) \\frac{h}{2} \\phi_1 \\left(-\\lambda \\frac{h}{2} \\right), \\\\\n",
    "  a_k = e^{-h \\lambda}y(t_k) + g(y(t_k), t_k) h \\phi_1 (-\\lambda h).\n",
    "$$"
   ]
  }
 ],
 "metadata": {
  "kernelspec": {
   "display_name": "Python 3",
   "language": "python",
   "name": "python3"
  },
  "language_info": {
   "codemirror_mode": {
    "name": "ipython",
    "version": 3
   },
   "file_extension": ".py",
   "mimetype": "text/x-python",
   "name": "python",
   "nbconvert_exporter": "python",
   "pygments_lexer": "ipython3",
   "version": "3.10.12"
  },
  "orig_nbformat": 4
 },
 "nbformat": 4,
 "nbformat_minor": 2
}
