{
 "cells": [
  {
   "attachments": {},
   "cell_type": "markdown",
   "metadata": {},
   "source": [
    "# Exponential methods"
   ]
  },
  {
   "attachments": {},
   "cell_type": "markdown",
   "metadata": {},
   "source": [
    "In this chapter, exponential methods are introduced, with further analysis of some of them, being tested and compared to more classical equivalents."
   ]
  },
  {
   "attachments": {},
   "cell_type": "markdown",
   "metadata": {},
   "source": [
    "## Exponential Euler method"
   ]
  },
  {
   "attachments": {},
   "cell_type": "markdown",
   "metadata": {},
   "source": [
    "For\n",
    "\n",
    "$\\begin{cases}\n",
    "    y'(t) + \\lambda y(t) = g(y(t), t), t \\in (t_0, T) \\\\\n",
    "    y(0) = y_0\n",
    "\\end{cases}$\n",
    "\n",
    "the domain is evenly discretized:\n",
    "\n",
    "$$\n",
    "    N \\in \\mathbb{N}; h = \\frac{T-t_0}{N}; \\text{Domain: }\\{t_k = t_0 + k h : k = 0, 1, ...\\}.\n",
    "$$\n",
    "\n",
    "The discretization of the ODE takes the exact solution of the Cauchy problem, given by the variation of constants formula\n",
    "\n",
    "$$\n",
    "    y(t) = e^{-(t-t_0) \\lambda}y_0 + \\int_{t_0}^t [e^{-\\lambda(t-\\tau)} g(y(\\tau), \\tau)] d\\tau\n",
    "$$\n",
    "\n",
    "and, by Taylor expansion on $g$:\n",
    "\n",
    "$\\tau \\in (t_k, t_{k+1})$\n",
    "\n",
    "$$\n",
    "    g(y(\\tau), \\tau) = g(y(t_k), t_k) + (\\tau - t_k) \\frac{dg}{dt} (y(\\theta_k), \\theta_k)\n",
    "$$\n",
    "\n",
    "for a $\\theta_k \\in (t_k, t_{k+1}),$\n",
    "\n",
    "$$\n",
    "    y(t_{k+1}) = e^{-(t_{k+1}-t_k) \\lambda}y(t_k) + \\int_{t_k}^{t_{k+1}} [e^{-\\lambda(t_{k+1}-\\tau)} g(y(\\tau), \\tau)] d\\tau\n",
    "$$\n",
    "\n",
    "$$\n",
    "    = e^{-h \\lambda}y(t_k) + \\int_{t_k}^{t_{k+1}} \\left[e^{-\\lambda(t_{k+1}-\\tau)} \\left( g(y(t_k), t_k) + (\\tau - t_k) \\frac{dg}{dt} (y(\\theta_k), \\theta_k)\\right)\\right] d\\tau\n",
    "$$\n",
    "\n",
    "$$\n",
    "    = e^{-h \\lambda}y(t_k) + g(y(t_k), t_k) \\int_{t_k}^{t_{k+1}} e^{-\\lambda(t_{k+1}-\\tau)} d\\tau + \\frac{dg}{dt} (y(\\theta_k), \\theta_k) \\int_{t_k}^{t_{k+1}} (\\tau - t_k) e^{-\\lambda(t_{k+1}-\\tau)} d\\tau.\n",
    "$$\n",
    "\n",
    "Since\n",
    "\n",
    "$$\n",
    "    \\int_{t_k}^{t_{k+1}} e^{-\\lambda(t_{k+1}-\\tau)} d\\tau = h\\phi_1(-\\lambda h)= \\frac{1-e^{-h \\lambda}}{\\lambda}\n",
    "$$\n",
    "\n",
    "and, by the Taylor expansion of $e^{-\\lambda h}$ in the point zero\n",
    "\n",
    "$$\n",
    "    e^{-\\lambda h} = 1 - \\lambda h + \\frac{1}{2}\\lambda^2h^2 - \\frac{1}{3!}\\lambda^3h^3 + \\dotsi + \\frac{1}{n!} (-\\lambda h)^n + \\dotsi, n \\in \\mathbb{N}\n",
    "$$\n",
    "\n",
    "$$\n",
    "     \\int_{t_k}^{t_{k+1}} (\\tau - t_k) e^{-\\lambda(t_{k+1}-\\tau)} d\\tau =\n",
    "     h^2 \\phi_2 (-\\lambda h) =\n",
    "     h \\frac{\\phi_1(0) - \\phi_1(-\\lambda h)}{\\lambda} =\n",
    "     \\frac{h}{\\lambda} - \\frac{1-e^{-h \\lambda}}{\\lambda^2} = \\\\\n",
    "     \\frac{h}{\\lambda} - \\frac{1-(1 - \\lambda h + \\frac{1}{2}\\lambda^2h^2 - \\frac{1}{3!}\\lambda^3h^3 + \\dotsi + \\frac{1}{n!} (-\\lambda h)^n + \\dotsi)}{\\lambda^2} = \\\\\n",
    "     \\frac{h^2}{2} - \\frac{h^3}{3!} \\lambda + \\dotsi + \\frac{h^n}{n!} (-\\lambda)^{n-2} + \\dotsi  =  O(h^2),\n",
    "$$\n",
    "\n",
    "$$\n",
    "    y(t_{k+1}) = e^{-h \\lambda}y(t_k) + g(y(t_k), t_k) \\frac{1-e^{-h \\lambda}}{\\lambda} + \\frac{dg}{dt} (y(\\theta_k), \\theta_k) O(h^2),\n",
    "$$\n",
    "\n",
    "$$\n",
    "  y(t_{k+1}) = e^{-h \\lambda}y(t_k) + g(y(t_k), t_k) \\frac{1-e^{-h \\lambda}}{\\lambda} + O(h^2).\n",
    "$$\n",
    "\n",
    "That inspires the $\\textbf{Exponential Euler method}$ :\n",
    "\n",
    "$$\n",
    "y_0 = y(t_0)\\\\\n",
    "\\textbf{for } k = 0, 1, 2, ..., N-1 :\\\\\n",
    "    y_{k+1} = e^{-h \\lambda}y_k + g(y_k, t_k) \\frac{1-e^{-h \\lambda}}{\\lambda}\\\\\n",
    "    t_{k+1} = t_k + h\n",
    "$$\n",
    "\n",
    "with $y_k \\thickapprox y(t_k)$."
   ]
  },
  {
   "attachments": {},
   "cell_type": "markdown",
   "metadata": {},
   "source": [
    "## Exponential time differencing methods (ETD)\n",
    "\n",
    "In the same conditions as above, it is taken a general Taylor expansion of $g$:\n",
    "\n",
    "$\\tau \\in (t_k, t_{k+1}), n \\in \\mathbb{N}$\n",
    "\n",
    "$$\n",
    "    g(y(\\tau), \\tau) = g(y(t_k), t_k) + (\\tau - t_k) \\frac{dg}{dt} (y(t_k), t_k) + \\frac{(\\tau - t_k)^2}{2!} \\frac{d^2g}{dt^2} (y(t_k), t_k) + \\\\\n",
    "    \\dotsi + \\frac{(\\tau - t_k)^{n-1}}{(n-1)!} \\frac{d^{n-1}g}{dt^{n-1}} (y(t_k), t_k) + \\frac{(\\tau - t_k)^n}{n!} \\frac{d^ng}{dt^n} (y(\\theta_k), \\theta_k)\n",
    "$$\n",
    "\n",
    "for a $\\theta_k \\in (t_k, t_{k+1})$\n",
    "\n",
    "In\n",
    "\n",
    "$$\n",
    "    y(t_{k+1}) = e^{-h \\lambda}y(t_k) + \\int_{t_k}^{t_{k+1}} e^{-\\lambda(t_{k+1}-\\tau)} g(y(\\tau), \\tau) d\\tau\n",
    "$$\n",
    "\n",
    "It will now become\n",
    "\n",
    "$$\n",
    "y(t_{k+1}) = e^{-h \\lambda}y(t_k) + \\int_{t_k}^{t_{k+1}} e^{-\\lambda(t_{k+1}-\\tau)}  g(y(t_k), t_k) +\n",
    "(\\tau - t_k) \\frac{dg}{dt} (y(t_k), t_k) +\n",
    "$$\n",
    "\n",
    "$$\n",
    " \\frac{(\\tau - t_k)^2}{2!} \\frac{d^2g}{dt^2} (y(t_k), t_k) + \\dotsi + \n",
    "$$\n",
    "\n",
    "$$\n",
    " + \\frac{(\\tau - t_k)^{n-1}}{(n-1)!} \\frac{d^{n-1}g}{dt^{n-1}} (y(t_k), t_k) + \\frac{(\\tau - t_k)^n}{n!} \\frac{d^ng}{dt^n} (y(\\theta_k), \\theta_k)  d\\tau,\n",
    "$$\n",
    "\n",
    "$$\n",
    "y(t_{k+1}) = e^{-h \\lambda}y(t_k) +\n",
    "g(y(t_k), t_k)\\int_{t_k}^{t_{k+1}} e^{-\\lambda(t_{k+1}-\\tau)} d \\tau +\n",
    "$$\n",
    "\n",
    "$$\n",
    "+ \\frac{dg}{dt}(y(t_k), t_k)\\int_{t_k}^{t_{k+1}} e^{-\\lambda(t_{k+1}-\\tau)} (\\tau - t_k)d\\tau + \\frac{d^2g}{dt^2} (y(t_k), t_k)\\int_{t_k}^{t_{k+1}} e^{-\\lambda(t_{k+1}-\\tau)} \\frac{(\\tau - t_k)^2}{2!}d\\tau +\n",
    "$$\n",
    "\n",
    "$$\n",
    "+ \\dotsi +\n",
    "$$\n",
    "\n",
    "$$\n",
    "+ \\frac{d^{n-1}g}{dt^{n-1}} (y(t_k), t_k)\\int_{t_k}^{t_{k+1}}  e^{-\\lambda(t_{k+1}-\\tau)} \\frac{(\\tau - t_k)^{n-1}}{(n-1)!} d\\tau + \\frac{d^ng}{dt^n} (y(\\theta_k), \\theta_k) \\int_{t_k}^{t_{k+1}}  e^{-\\lambda(t_{k+1}-\\tau)} \\frac{(\\tau - t_k)^n}{n!} d\\tau,\n",
    "$$\n",
    "\n",
    "$$\n",
    "y(t_{k+1}) = e^{-h \\lambda}y(t_k) +\n",
    "h\\phi_1(-\\lambda h) g(y(t_k), t_k) +\n",
    "h^2\\phi_2(-\\lambda h) \\frac{dg}{dt}(y(t_k), t_k) +\n",
    "h^3\\phi_3(-\\lambda h)\\frac{d^2g}{dt^2} (y(t_k), t_k)\n",
    "$$\n",
    "\n",
    "$$\n",
    "+ \\dotsi +\n",
    "$$\n",
    "\n",
    "$$\n",
    "+ h^n\\phi_n(-\\lambda h) \\frac{d^{n-1}g}{dt^{n-1}} (y(t_k), t_k)+\n",
    "h^{n+1}\\phi_{n+1}(-\\lambda h) \\frac{d^ng}{dt^n} (y(\\theta_k), \\theta_k).\n",
    "$$\n",
    "\n",
    "From the discussion about the exponential Euler, that is known that\n",
    "\n",
    "$$\n",
    "h^2\\phi_2(-\\lambda h) = \\frac{h^2}{2} - \\frac{h^3}{3!} \\lambda + \\dotsi + \\frac{h^l}{l!} (-\\lambda)^{l-2} + \\dotsi = \\frac{1}{(-\\lambda)^2} \\sum\\limits_{i=2}^{\\infty} \\frac{(-\\lambda h)^i}{i!}.\n",
    "$$\n",
    "\n",
    "Since\n",
    "\n",
    "$$\n",
    "  \\phi_{n+1}(-\\lambda h) = \\frac{\\phi_n(-\\lambda h) - \\phi_n(0)}{-\\lambda h} \\text{ and}\\\\\n",
    "  \\phi_n(0) = \\frac{1}{n!},\n",
    "$$\n",
    "\n",
    "$$\n",
    "  h^3 \\phi_3(-\\lambda h) = h^2 \\frac{\\phi_2(0) - \\phi_2(-\\lambda h)}{\\lambda} = \\frac{\\frac{h^2}{2} - (\\frac{h^2}{2} - \\frac{h^3}{3!} \\lambda + \\dotsi + \\frac{h^l}{l!} (-\\lambda)^{l-2} + O(h^{l+1}))}{\\lambda} = \\frac{1}{(-\\lambda)^3} \\sum\\limits_{i=3}^{\\infty} \\frac{(-\\lambda h)^i}{i!}.\n",
    "$$\n",
    "\n",
    "And if\n",
    "\n",
    "$$\n",
    "h^l \\phi_l(-\\lambda h) = \\frac{1}{(-\\lambda)^l} \\sum\\limits_{i=l}^{\\infty} \\frac{(-\\lambda h)^i}{i!}, \\text{for a } l \\in \\mathbb{N},\n",
    "$$\n",
    "\n",
    "$$\n",
    "  h^{l+1}\\phi_{l+1}(-\\lambda h) = h^{l+1} \\frac{\\phi_l(-\\lambda h) - \\phi_l(0)}{-\\lambda h} = \\frac{h^l \\phi_l(0) - h^l \\phi_l(-\\lambda h)}{\\lambda} = \\frac{h^l}{l! \\lambda} - \\frac{1}{\\lambda} \\frac{1}{(-\\lambda)^l} \\sum\\limits_{i=l}^{\\infty} \\frac{(-\\lambda h)^i}{i!} = \\frac{1}{(-\\lambda)^{l+1}} \\sum\\limits_{i=l+1}^{\\infty} \\frac{(-\\lambda h)^i}{i!}.\n",
    "$$\n",
    "\n",
    "So, by induction,\n",
    "\n",
    "$$\n",
    "h^n \\phi_n(-\\lambda h) = \\frac{1}{(-\\lambda)^n} \\sum\\limits_{i=n}^{\\infty} \\frac{(-\\lambda h)^i}{i!} = O(h^n), \\forall n \\geq 2.\n",
    "$$"
   ]
  },
  {
   "attachments": {},
   "cell_type": "markdown",
   "metadata": {},
   "source": [
    "Then,\n",
    "\n",
    "$$\n",
    "y(t_{k+1}) = e^{-h \\lambda}y(t_k) +\n",
    "h\\phi_1(-\\lambda h) g(y(t_k), t_k) +\n",
    "h^2\\phi_2(-\\lambda h) \\frac{dg}{dt}(y(t_k), t_k) +\n",
    "h^3\\phi_3(-\\lambda h)\\frac{d^2g}{dt^2} (y(t_k), t_k) +\n",
    "\\dotsi + \\\\\n",
    "h^n\\phi_n(-\\lambda h) \\frac{d^{n-1}g}{dt^{n-1}} (y(t_k), t_k)+\n",
    "O(h^{n+1}).\n",
    "$$"
   ]
  },
  {
   "attachments": {},
   "cell_type": "markdown",
   "metadata": {},
   "source": [
    "It is possible to note that the exponential euler is essentially the exponential time differencing method of order 1.\n",
    "\n",
    "In the same way as Taylor methods, the problem here is that at the expense of a higher order of convergence, ends up requiring the evaluation and implementation of multiple derivatives that may not even be easy to calculate. It can be avoided using Runge-Kutta methods."
   ]
  },
  {
   "attachments": {},
   "cell_type": "markdown",
   "metadata": {},
   "source": [
    "## Exponential time differencing methods with Runge-Kutta time stepping\n",
    "\n",
    "For the Runge-Kutte methods, that is used approximations of the derivatives that converges together with the whole expression as the time step decreases."
   ]
  }
 ],
 "metadata": {
  "kernelspec": {
   "display_name": "Python 3",
   "language": "python",
   "name": "python3"
  },
  "language_info": {
   "codemirror_mode": {
    "name": "ipython",
    "version": 3
   },
   "file_extension": ".py",
   "mimetype": "text/x-python",
   "name": "python",
   "nbconvert_exporter": "python",
   "pygments_lexer": "ipython3",
   "version": "3.10.6"
  }
 },
 "nbformat": 4,
 "nbformat_minor": 2
}